Lemma 6: refactor start

src/AuxDef.v
@@ -2,9 +2,17 @@ From imm Require Import Events Execution imm_s_hb.
 From imm Require Import imm_s_ppo.
 From imm Require Import imm_s_hb.
 From imm Require Import imm_bob.
+From imm Require Import SubExecution.
+
+Require Import Program.Basics.
 
 From hahn Require Import Hahn.
 From hahnExt Require Import HahnExt.
+From PromisingLib Require Import Language Basic.
+
+Open Scope program_scope.
+
+Set Implicit Arguments.
 
 Section HbAlt.
 
@@ -228,3 +236,212 @@ Proof using.
   unfold sb in RMW. unfolder in RMW.
   desf.
 Qed.
+
+Lemma list_min_elt {A} {h : A} {t}
+    (NODUP : NoDup (h :: t)) :
+  min_elt (total_order_from_list (h :: t)) h.
+Proof using.
+  unfolder. unfold total_order_from_list.
+  intros e F. desf.
+  enough (IN : In h t) by inv NODUP.
+  destruct l1 as [ | h' t']; inv F.
+  { apply in_app_iff. right. desf. }
+  apply in_app_iff; right.
+  ins. right.
+  apply in_app_iff. right.
+  now left.
+Qed.
+
+Lemma equiv_seq_eq {A} (s : A -> Prop)
+  (r : relation A) :
+  ⦗s⦘ ⨾ (⦗s⦘ ⨾ r ⨾ ⦗s⦘) ⨾ ⦗s⦘ ≡ ⦗s⦘ ⨾ r ⨾ ⦗s⦘.
+Proof using.
+  basic_solver.
+Qed.
+
+Lemma in_restr_acts G e :
+  acts_set G e <-> (acts_set G ∩₁ same_tid e) e.
+Proof using.
+  unfolder; split; ins; desf.
+Qed.
+
+Section PartialId.
+
+Variable A : Type.
+Variable f : A -> option A.
+
+Definition partial_id := forall x y (SOME : f x = Some y), y = x.
+
+Hypothesis PARTIAL : partial_id.
+
+
+Lemma partial_id_iff x : (is_some ∘ f) x <-> f x = Some x.
+Proof using PARTIAL.
+  unfold compose, is_some.
+  split; ins; desf.
+  f_equal. now apply PARTIAL.
+Qed.
+
+Lemma partial_id_rel r : Some ↓ (f ↑ r) ≡ restr_rel (is_some ∘ f) r.
+Proof using PARTIAL.
+  symmetry. unfolder; splits; ins; desf.
+  { do 2 eexists. rewrite <- !partial_id_iff; auto. }
+  rewrite PARTIAL with (x := x') (y := x),
+          PARTIAL with (x := y') (y := y).
+  all: splits; auto.
+  all: unfold is_some, compose; desf.
+Qed.
+
+Lemma partial_id_set s : Some ↓₁ (f ↑₁ s) ≡₁ s ∩₁ (is_some ∘ f).
+Proof using PARTIAL.
+  symmetry.
+  unfolder. splits; ins; desf.
+  { eexists. rewrite <- !partial_id_iff; auto. }
+  rewrite PARTIAL with (x := y) (y := x); auto.
+  all: unfold is_some, compose; desf.
+Qed.
+
+Lemma partial_id_inj s :
+  inj_dom (s ∩₁ (is_some ∘ f)) f.
+Proof using PARTIAL.
+  unfolder; ins; desf.
+  apply PARTIAL. rewrite <- EQ.
+  now apply partial_id_iff.
+Qed.
+
+Lemma partial_id_sub_eq :
+  (fun x y => f x = Some y) ⊆ (fun x => eq x).
+Proof using PARTIAL.
+  unfolder; ins; desf.
+  symmetry; now apply PARTIAL.
+Qed.
+
+End PartialId.
+
+Section SubFunction.
+
+Definition sub_fun {A B} (f g : A -> option B) :=
+  forall x y (SOME : f x = Some y), g x = Some y.
+
+Lemma sub_id_refl {A B} : reflexive (@sub_fun A B).
+Proof using.
+  now unfolder.
+Qed.
+
+Lemma sub_id_trans {A B} : transitive (@sub_fun A B).
+Proof using.
+  unfolder. unfold sub_fun.
+  intros f g h SUB1 SUB2 x y EQ.
+  now apply SUB1, SUB2 in EQ.
+Qed.
+
+Add Parametric Relation A B : (A -> option B) (@sub_fun A B)
+  reflexivity proved by (sub_id_refl (A:=A) (B:=B))
+  transitivity proved by (sub_id_trans (A:=A) (B:=B))
+  as sub_fun_rel.
+
+Add Parametric Morphism A : (@partial_id A) with signature
+  sub_fun --> Basics.impl as partial_id_mori.
+Proof using.
+  unfolder; unfold sub_fun, partial_id.
+  ins; auto.
+Qed.
+
+End SubFunction.
+
+Section ExecEqv.
+
+Variable (G G' : execution).
+Notation "'D'" := (acts_set G' \₁ acts_set G).
+
+Record exec_equiv : Prop := {
+  exeeqv_acts : acts_set G ≡₁ acts_set G';
+  exeeqv_threads : threads_set G ≡₁ threads_set G';
+  exeeqv_lab : lab G = lab G';
+  exeeqv_rmw : rmw G ≡ rmw G';
+  exeeqv_data : data G ≡ data G';
+  exeeqv_addr : addr G ≡ addr G';
+  exeeqv_ctrl : ctrl G ≡ ctrl G';
+  exeeqv_rmw_dep : rmw_dep G ≡ rmw_dep G';
+  exeeqv_rf : rf G ≡ rf G';
+  exeeqv_co : co G ≡ co G';
+}.
+
+Lemma exec_equiv_eq (EQV : exec_equiv) : G = G'.
+Proof using.
+  destruct EQV, G, G'; f_equal.
+  all: try apply set_extensionality.
+  all: try apply rel_extensionality.
+  all: assumption.
+Qed.
+
+Lemma sub_sub_equiv sc sc'
+    (WF : Wf G')
+    (SUB : sub_execution G G' sc sc')
+    (SUB' : sub_execution G' G sc' sc) :
+  exec_equiv.
+Proof using.
+  assert (HEQ : acts_set G ≡₁ acts_set G').
+  { split; eauto using sub_E. }
+  constructor; eauto using sub_lab, sub_threads.
+  all: rewrite 1?sub_rmw,
+    1?sub_data,
+    1?sub_addr,
+    1?sub_ctrl,
+    1?sub_frmw,
+    1?sub_rf,
+    1?sub_co at 1; eauto.
+  all: try rewrite HEQ.
+  all: now rewrite <- 1?wf_rmwE,
+    <- 1?wf_dataE,
+    <- 1?wf_addrE,
+    <- 1?wf_ctrlE,
+    <- 1?wf_rmw_depE,
+    <- 1?wf_rfE,
+    <- 1?wf_coE; auto.
+Qed.
+
+Lemma sub_sym
+    (WF_G : Wf G')
+    (PREFIX : sub_execution G' G ∅₂ ∅₂)
+    (ENUM_D : D ≡₁ ∅) :
+  sub_execution G G' ∅₂ ∅₂.
+Proof using.
+    assert (E_EQ : acts_set G = acts_set G').
+    { apply set_extensionality.
+      split; eauto using sub_E.
+      now apply set_subsetE. }
+    constructor.
+    all: try now symmetry; apply PREFIX.
+    all: try now rewrite seq_false_l, seq_false_r.
+    { now rewrite E_EQ. }
+    all: rewrite 1?wf_rmwE,
+                 1?wf_dataE,
+                 1?wf_addrE,
+                 1?wf_ctrlE,
+                 1?wf_rmw_depE,
+                 1?wf_rfE,
+                 1?wf_coE; auto.
+    all: symmetry.
+    all: rewrite 1?sub_rmw,
+                 1?sub_data,
+                 1?sub_addr,
+                 1?sub_ctrl,
+                 1?sub_frmw,
+                 1?sub_rf,
+                 1?sub_co; eauto.
+    all: rewrite E_EQ.
+    all: apply equiv_seq_eq.
+Qed.
+
+Lemma sub_eq
+    (WF_G : Wf G')
+    (PREFIX : sub_execution G' G ∅₂ ∅₂)
+    (ENUM_D : D ≡₁ ∅)
+     : G = G'.
+Proof using.
+  eapply exec_equiv_eq, sub_sub_equiv; eauto.
+  now apply sub_sym.
+Qed.
+
+End ExecEqv.
