src/Reordering.v
@@ -15,55 +15,390 @@ From imm Require Import imm_s_hb.
 From imm Require Import imm_bob.
 From imm Require Import SubExecution.
 
-Record exec_equiv G G' : Prop := {
-  exeeqv_acts : acts_set G ≡₁ acts_set G';
-  exeeqv_threads : threads_set G ≡₁ threads_set G';
-  exeeqv_lab : lab G = lab G';
-  exeeqv_rmw : rmw G ≡ rmw G';
-  exeeqv_data : data G ≡ data G';
-  exeeqv_addr : addr G ≡ addr G';
-  exeeqv_ctrl : ctrl G ≡ ctrl G';
-  exeeqv_rmw_dep : rmw_dep G ≡ rmw_dep G';
-  exeeqv_rf : rf G ≡ rf G';
-  exeeqv_co : co G ≡ co G';
+Section SubGraphLemma.
+
+Variable G G' : execution.
+Variable C : actid -> Prop.
+Variable traces : thread_id -> trace label -> Prop.
+
+Notation "'lab''" := (lab G').
+Notation "'E''" := (acts_set G').
+Notation "'rmw''" := (rmw G').
+Notation "'data''" := (data G').
+Notation "'addr''" := (addr G').
+Notation "'ctrl''" := (ctrl G').
+Notation "'rmw_dep''" := (rmw_dep G').
+Notation "'rf''" := (rf G').
+Notation "'co''" := (co G').
+Notation "'W''" := (fun x => is_w lab' x).
+Notation "'R''" := (fun x => is_r lab' x).
+
+Notation "'lab'" := (lab G).
+Notation "'E'" := (acts_set G).
+Notation "'rmw'" := (rmw G).
+Notation "'data'" := (data G).
+Notation "'addr'" := (addr G).
+Notation "'ctrl'" := (ctrl G).
+Notation "'rmw_dep'" := (rmw_dep G).
+Notation "'rf'" := (rf G).
+Notation "'co'" := (co G).
+Notation "'W'" := (fun x => is_w lab x).
+Notation "'R'" := (fun x => is_r lab x).
+
+Lemma over_exec_wf f
+    (WF : Wf G')
+    (F_ID : partial_id f)
+    (CTRL : ctrl' ≡ ∅₂)
+    (ADDR : addr' ≡ ∅₂)
+    (DATA : data' ≡ ∅₂)
+    (A_CORRECT : is_some ∘ f ⊆₁ E)
+    (C_CORRECT : C ⊆₁ is_some ∘ f)
+    (SUB_INIT : E' ∩₁ is_init ⊆₁ E)
+    (G_RF_D : E ∩₁ R ⊆₁ codom_rel rf ∪₁ (Some ↓₁ (f ↑₁ C)))
+    (G_TIDS : (tid ↓₁ eq tid_init) ∩₁ E' ⊆₁ is_init)
+    (G_ACTS : forall thr (NOT_INIT : thr <> tid_init),
+      exists N, E ∩₁ (fun x => thr = tid x) ≡₁ thread_seq_set thr N)
+    (SUB : sub_execution G' G ∅₂ ∅₂) :
+  WCore.wf (WCore.Build_t G G' C f).
+Proof using.
+  assert (ACT_SUB : E ⊆₁ E').
+  { apply SUB. }
+  constructor; ins.
+  { rewrite sub_ctrl, CTRL; eauto; basic_solver. }
+  { rewrite sub_addr, ADDR; eauto; basic_solver. }
+  { rewrite sub_data, DATA; eauto; basic_solver. }
+  { eapply sub_WF; eauto. now rewrite set_interC. }
+  { now rewrite ACT_SUB. }
+  { transitivity E; auto. }
+  { rewrite partial_id_set; eauto; basic_solver. }
+  { now apply partial_id_inj. }
+  { rewrite sub_sb with (G' := G), partial_id_rel, !restr_relE; eauto.
+    basic_solver. }
+  { rewrite sub_rf with (G' := G), partial_id_rel, !restr_relE; eauto.
+    basic_solver. }
+  { rewrite partial_id_sub_eq; auto; basic_solver. }
+  { unfold WCore.unwrap_g2gc, same_lab_u2v_dom,
+          is_some, compose.
+    unfolder. ins. desf.
+    erewrite sub_lab, (F_ID e a); eauto.
+    red. desf. }
+  apply C_CORRECT, partial_id_iff in IN; auto.
+  unfold WCore.unwrap_g2gc, val.
+  erewrite sub_lab; eauto.
+  ins. now rewrite IN.
+Qed.
+
+End SubGraphLemma.
+
+Section ReorderingSubLemma.
+
+(* G ⊂ G' *)
+Definition delta_G G G' e :=
+  {| acts_set := acts_set G ∪₁ eq e;
+     threads_set := threads_set G;
+     lab := lab G;
+     rmw := rmw G ∪ (⦗acts_set G⦘ ⨾ (rmw G') ⨾ ⦗eq e⦘);
+     data := ∅₂;
+     addr := ∅₂;
+     ctrl := ∅₂;
+     rmw_dep := ⦗acts_set G ∪₁ eq e⦘ ⨾ rmw_dep G' ⨾ ⦗acts_set G ∪₁ eq e⦘;
+     rf := rf G ∪ (⦗acts_set G⦘ ⨾ (rf G') ⨾ ⦗eq e⦘) ∪
+                  (⦗eq e⦘ ⨾ (rf G') ⨾ ⦗acts_set G⦘);
+     co := co G ∪ (⦗acts_set G⦘ ⨾ (co G') ⨾ ⦗eq e⦘) ∪
+                  (⦗eq e⦘ ⨾ (co G') ⨾ ⦗acts_set G⦘);
+  |}.
+
+
+Variable G G' : execution.
+Variable C : actid -> Prop.
+Variable traces : thread_id -> trace label -> Prop.
+
+Notation "'lab''" := (lab G').
+Notation "'E''" := (acts_set G').
+Notation "'sb''" := (sb G').
+Notation "'rmw''" := (rmw G').
+Notation "'data''" := (data G').
+Notation "'addr''" := (addr G').
+Notation "'ctrl''" := (ctrl G').
+Notation "'rmw_dep''" := (rmw_dep G').
+Notation "'rf''" := (rf G').
+Notation "'co''" := (co G').
+Notation "'W''" := (fun x => is_w lab' x).
+Notation "'R''" := (fun x => is_r lab' x).
+
+Notation "'lab'" := (lab G).
+Notation "'E'" := (acts_set G).
+Notation "'rmw'" := (rmw G).
+Notation "'data'" := (data G).
+Notation "'addr'" := (addr G).
+Notation "'ctrl'" := (ctrl G).
+Notation "'rmw_dep'" := (rmw_dep G).
+Notation "'rf'" := (rf G).
+Notation "'co'" := (co G).
+Notation "'W'" := (fun x => is_w lab x).
+Notation "'R'" := (fun x => is_r lab x).
+
+(* TODO: remove *)
+Notation "'U'" := (E' \₁ C).
+Notation "'D'" := (E' \₁ E).
+
+Lemma delta_G_sub e f
+    (NOT_INIT : tid e <> tid_init)
+    (WF : WCore.wf (WCore.Build_t G G' C f))
+    (IN : E' e)
+    (NEW : ~E e)
+    (SUB : sub_execution G' G ∅₂ ∅₂) :
+  sub_execution G' (delta_G G G' e) ∅₂ ∅₂.
+Proof using.
+  assert (WF' : Wf G').
+  { apply WF. }
+  assert (SUBE : E ⊆₁ E').
+  { apply SUB. }
+  constructor; ins.
+  all: try apply SUB.
+  { unfolder. ins. desf. now apply SUB. }
+  { rewrite !id_union, seq_union_l,
+            !seq_union_r, <- (sub_rmw SUB).
+    rewrite one_dir_irrefl; eauto using rmw_one_dir.
+    destruct (classic (dom_rel (rmw' ⨾ ⦗E⦘) e)) as [HIN1|HIN1].
+    { rewrite one_dir_assym_1, !union_false_r;
+        eauto using rmw_one_dir, one_dir_dom.
+      unfolder in HIN1. desf.
+      enough (EINE : E e).
+      { arewrite (⦗eq e⦘ ≡ ⦗eq e⦘ ⨾ ⦗E⦘); try basic_solver. }
+      apply wf_rmwi, immediate_in in HIN1; eauto.
+      change E with (acts_set (WCore.G {|
+        WCore.G := G;
+        WCore.GC := G';
+        WCore.cmt := C;
+        WCore.g2gc := f
+      |})).
+      eapply WCore.ext_sb_dense; eauto.
+      unfold sb in HIN1. unfolder in HIN1.
+      desf. }
+    destruct (classic (codom_rel (⦗E⦘ ⨾ rmw') e)) as [HIN2|HIN2].
+    { rewrite one_dir_assym_2, !union_false_r;
+      eauto using rmw_one_dir, one_dir_dom. }
+    rewrite one_dir_assym_helper_1, one_dir_assym_helper_2,
+            !union_false_r; eauto. }
+  { rewrite (WCore.cc_data_empty WF); basic_solver. }
+  { rewrite (WCore.cc_addr_empty WF); basic_solver. }
+  { rewrite (WCore.cc_ctrl_empty WF); basic_solver. }
+  { rewrite !id_union, seq_union_l,
+            !seq_union_r, <- (sub_rf SUB).
+    rewrite one_dir_irrefl; eauto using rf_one_dir.
+    now rewrite union_false_r. }
+  { rewrite !id_union, seq_union_l,
+            !seq_union_r, <- (sub_co SUB).
+    arewrite (⦗eq e⦘ ⨾ co' ⨾ ⦗eq e⦘ ≡ ∅₂); [| now rewrite union_false_r].
+    split; [| basic_solver].
+    unfolder; ins; desf.
+    eapply co_irr; eauto. }
+  basic_solver.
+Qed.
+
+Hypothesis THREAD_EVENTS : forall t, exists N,
+  E' ∩₁ (fun e => t = tid e) ≡₁ thread_seq_set t N.
+
+Record reord_lemma_enum (E E' C : actid -> Prop) l : Prop :=
+{ relenum_nodup : NoDup l;
+  relenum_no_init : (fun x => In x l) ⊆₁ set_compl (fun a => is_init a);
+  relenum_d : (fun x => In x l) ≡₁ D;
+  relenum_sb : restr_rel (fun x => In x l) sb' ⊆ total_order_from_list l;
+  (* C substraction seems to be redundant *)
+  relenum_rf : restr_rel (fun x => In x l) rf' ⨾ ⦗E' \₁ C⦘ ⊆ total_order_from_list l;
+  relenum_rf_w : dom_rel (rf' ⨾ ⦗fun x => In x l⦘) ⊆₁ E ∪₁ fun x => In x l;
 }.
 
-Lemma exec_equiv_eq G G'
-  (EQV : exec_equiv G G') :
-  G = G'.
+(* Lemma new_event_not_in_C e f
+    (WF : WCore.wf (WCore.Build_t G G' C f))
+    (NEW : D e) :
+  ~(Some ↓₁ (f ↑₁ C)) e.
 Proof using.
-  destruct EQV, G, G'; f_equal.
-  all: try apply set_extensionality.
-  all: try apply rel_extensionality.
-  all: assumption.
+  intro IN_C.
+  enough (E e) by now apply NEW.
+  apply (WCore.f_codom WF).
+  enough (Some ↓₁ (f ↑₁ C) ⊆₁ Some ↓₁ (f ↑₁ E')) by auto.
+  apply set_map_mori, set_subset_collect; eauto.
+  apply (WCore.C_sub_EC WF).
+Qed. *)
+
+Lemma reord_lemma_enum_head h t
+    (ENUM : reord_lemma_enum E E' C (h :: t))
+    (NOT_CMT : ~C h) :
+  dom_rel (rf' ⨾ ⦗eq h⦘) ⊆₁ E.
+Proof using.
+  intros e IN.
+  edestruct (relenum_rf_w E E' C (h :: t) ENUM) as [EIN|EIN]; eauto.
+  { enough (SUB : eq e ⊆₁ dom_rel (rf' ⨾ ⦗fun x => In x (h :: t)⦘)).
+    { now apply SUB. }
+    transitivity (dom_rel (rf' ⨾ ⦗eq h⦘)); [| basic_solver].
+    red; ins; desf. }
+  exfalso. enough (LT : total_order_from_list (h::t) e h).
+  { eapply list_min_elt; [apply ENUM | apply LT]. }
+  apply (relenum_rf E E' C (h :: t) ENUM).
+  unfolder; split.
+  { unfolder in IN; desf. }
+  split; eauto.
+  apply ENUM; desf.
 Qed.
 
-Lemma sub_sub_equiv sc sc' G G'
-  (WF : Wf G')
-  (SUB : sub_execution G G' sc sc')
-  (SUB' : sub_execution G' G sc' sc) :
-  exec_equiv G G'.
-Proof using.
-  assert (HEQ : acts_set G ≡₁ acts_set G').
-  { split; eauto using sub_E. }
-  constructor; eauto using sub_lab, sub_threads.
-  all: rewrite 1?sub_rmw,
-    1?sub_data,
-    1?sub_addr,
-    1?sub_ctrl,
-    1?sub_frmw,
-    1?sub_rf,
-    1?sub_co at 1; eauto.
-  all: try rewrite HEQ.
-  all: now rewrite <- 1?wf_rmwE,
-    <- 1?wf_dataE,
-    <- 1?wf_addrE,
-    <- 1?wf_ctrlE,
-    <- 1?wf_rmw_depE,
-    <- 1?wf_rfE,
-    <- 1?wf_coE; auto.
-Qed.
+(* NOTE: do not change threads_set! It must remain constant *)
+(* TODO: either rename or move into module *)
+Lemma step_once_read h t f f'
+    (F_ID : partial_id f')
+    (SUB_ID : sub_fun f f')
+    (WF : WCore.wf (WCore.Build_t G G' C f))
+    (WF' : WCore.wf (WCore.Build_t G' G' C f'))
+    (PREFIX : restr_exec E G' G)
+    (ENUM : reord_lemma_enum E E' C (h :: t))
+    (COH : trace_coherent traces G')
+    (IS_R : R' h) :
+  WCore.cfg_add_step_uninformative traces
+    (WCore.Build_t G                G' C f)
+    (WCore.Build_t (delta_G G G' h) G' C (upd f h (Some h))).
+Proof using THREAD_EVENTS.
+  (* Information about h *)
+  assert (IN_D : D h).
+  { apply ENUM; desf. }
+  destruct (classic (C h)) as [INC|INC].
+  (* CASE 1: h is cmt *)
+  { admit. (*TODO*) }
+  edestruct WCore.f_rfD with (X := WCore.Build_t G' G' C f') (x := h)
+    as [[w RF] | CMT]; ins.
+  { split; [apply IN_D | auto]. }
+  2: admit. (* show that then h is in C *)
+  assert (W_IN_E : E w).
+  { eapply reord_lemma_enum_head; eauto.
+    unfolder. eauto. }
+  exists h, (lab' h), None, (Some w), ∅, ∅, (Some h).
+  constructor; ins.
+  all: admit.
+(****************)
+  (* assert (IN_D : D h).
+  { apply ENUM; now constructor. }
+  assert (NOT_W : ~ W' h).
+  { generalize IS_R. unfold is_w, is_r.
+    now destruct (lab' h). }
+  assert (R_IN_G' : (E' ∩₁ R') h).
+  { split; try apply IN_D; eauto. }
+  destruct (WCore.f_rfD WF' R_IN_G') as [RF | CMT]; ins.
+  all: try now (exfalso; eapply new_event_not_in_C with (f := f); eauto).
+  destruct RF as [w RF]; ins.
+  assert (W_IN_E : E w).
+  { eapply reord_lemma_enum_head; eauto.
+    { intro F. eapply new_event_not_in_C with (f := f); eauto.
+      apply partial_id_set; eauto.  }
 
+
+  set (G'' := delta_G G G' h).
+  assert (G_SB_SUB : sb G ⊆ sb G'').
+  { unfold sb; subst G''; ins. basic_solver 2. }
+  assert (IS_W : W' w).
+  { eapply wf_rfD in RF; try now apply WF. unfolder in RF; desf. }
+  exists (upd f h (Some h)), G'',
+          h, (lab' h),
+          None, (Some w), ∅, ∅, (Some h).
+  constructor.
+  all: try easy.
+  all: ins; desf.
+  { apply IN_D. }
+  { apply ENUM; now constructor. }
+  { admit. }
+  { erewrite sub_lab with (G := G'); try apply PREFIX.
+    apply functional_extensionality; ins.
+    destruct (classic (x = h)) as [EQ|NEQ]; subst.
+    all: now rupd. }
+  { apply union_more; [apply union_more; auto |].
+    { admit. }
+    rewrite wf_rfD, seqA; try apply WF.
+    unfold WCore.rf_delta_W.
+    arewrite (⦗eq h⦘ ⨾ ⦗W'⦘ ≡ ∅₂); try basic_solver.
+    rewrite seq_false_l.
+    arewrite (upd f h (Some h) ↓₁ eq (Some h) ≡₁ eq h).
+    { unfolder; split; intros x HEQ; subst.
+      { destruct (classic (h = x)) as [EQ|NEQ]; auto.
+        rewrite updo in HEQ; auto. }
+      now rewrite upds. }
+    arewrite (⦗eq h⦘ ⨾ rf' ≡ ∅₂).
+    { rewrite wf_rfD; try apply WF'.
+      basic_solver. }
+    basic_solver. }
+  { admit. }
+  { admit. }
+  apply over_exec_wf.
+  all: try apply WF'.
+  { intros x y.
+    destruct (classic (x = h)) as [EQ|NEQ]; desf.
+    { rewrite upds; congruence. }
+    rewrite updo; auto. }
+  { unfolder. unfold is_some, compose. ins.
+    destruct (classic (x = h)) as [EQ|NEQ]; desf.
+    { now right. }
+    rewrite updo in Heq; auto.
+    left. apply (WCore.f_codom WF). ins.
+    assert (ID : f x = Some x) by now rewrite <- (F_ID x a) at 2.
+    exists x. split; [apply WF, partial_id_iff |]; auto. }
+  { transitivity (is_some ∘ f); try apply WF.
+    unfolder. unfold is_some, compose. ins.
+    destruct (classic (x = h)) as [EQ|NEQ]; desf.
+    { rewrite upds in Heq. congruence. }
+    rewrite updo in Heq; auto.
+    congruence. }
+  { subst G''. ins.
+    transitivity (E ∩₁ is_init); try apply PREFIX.
+    transitivity E; basic_solver. }
+  { subst G''. ins.
+    rewrite set_inter_union_l, codom_union.
+    admit.
+    (* split this into 2 refineable inclusions *) }
+  { subst G''. ins.
+    admit.
+    (* Infer it from trace coherency. *) }
+  subst G''. eapply delta_G_sub.
+  { admit. }
+  { apply WF. }
+  { apply IN_D. }
+  { apply IN_D. }
+  apply PREFIX. *)
+Admitted.
+
+Lemma step_once h t (f : actid -> option actid)
+  (WF : WCore.wf (WCore.Build_t G G' C f))
+  (PREFIX : restr_exec E G' G)
+  (C_SUB : C ⊆₁ E')
+  (VALID_ENUM : NoDup (h :: t))
+  (NOT_INIT : (fun x => In x (h :: t)) ⊆₁ set_compl is_init)
+  (ENUM_D : (fun x => In x (h :: t)) ≡₁ D)
+  (ORD_SB : restr_rel (fun x => In x (h :: t)) (sb G') ⊆ total_order_from_list (h :: t))
+  (ORD_RF : restr_rel (fun x => In x (h :: t)) rf' ⨾ ⦗U⦘ ⊆ total_order_from_list (h :: t)) :
+  exists f' G'',
+  (WCore.cfg_add_step_uninformative traces)
+  (WCore.Build_t G G' C f)
+  (WCore.Build_t G'' G' C f').
+Proof using.
+  eexists (upd f h (Some h)), _, h, (lab' h).
+  destruct (lab' h) eqn:HEQ_LAB.
+  all: admit.
+Admitted.
+
+(* Lemma steps l
+    (WF : Wf G)
+    (PREFIX : restr_exec E G' G)
+    (C_SUB : C ⊆₁ E')
+    (VALID_ENUM : NoDup l)
+    (ENUM_D : (fun x => In x l) ≡₁ D)
+    (ORD_SB : sb G' ⊆ enum_ord)
+    (ORD_RF : rf' ⨾ ⦗U⦘ ⊆ enum_ord) :
+    exists f',
+    (WCore.silent_cfg_add_step traces)＊
+    (WCore.Build_t G G' C f)
+    (WCore.Build_t G' G' C f').
+Proof using.
+  admit.
+Admitted. *)
+
+End ReorderingSubLemma.
 Section GraphDefs.
 
 Variable G : execution.
@@ -95,7 +430,6 @@ End GraphDefs.
 Section ReorderingDefs.
 
 Open Scope program_scope.
-
 
 Variable G G' : execution.
 Variable traces traces' : thread_id -> trace label -> Prop.
@@ -189,439 +523,6 @@ Record simrel_not_rw m : Prop :=
 }.
 
 End ReorderingDefs.
-
-Section SubGraphLemma.
-
-Variable G G' : execution.
-Variable C : actid -> Prop.
-Variable traces : thread_id -> trace label -> Prop.
-
-Notation "'lab''" := (lab G').
-Notation "'E''" := (acts_set G').
-Notation "'rmw''" := (rmw G').
-Notation "'data''" := (data G').
-Notation "'addr''" := (addr G').
-Notation "'ctrl''" := (ctrl G').
-Notation "'rmw_dep''" := (rmw_dep G').
-Notation "'rf''" := (rf G').
-Notation "'co''" := (co G').
-Notation "'W''" := (fun x => is_w lab' x).
-Notation "'R''" := (fun x => is_r lab' x).
-
-Notation "'lab'" := (lab G).
-Notation "'E'" := (acts_set G).
-Notation "'rmw'" := (rmw G).
-Notation "'data'" := (data G).
-Notation "'addr'" := (addr G).
-Notation "'ctrl'" := (ctrl G).
-Notation "'rmw_dep'" := (rmw_dep G).
-Notation "'rf'" := (rf G).
-Notation "'co'" := (co G).
-Notation "'W'" := (fun x => is_w lab x).
-Notation "'R'" := (fun x => is_r lab x).
-
-Lemma partial_id_iff {A} (f : A -> option A) x
-    (F_ID : forall x y (SOME : f x = Some y), y = x) :
-  (is_some ∘ f) x <-> f x = Some x.
-Proof using.
-  unfold compose, is_some.
-  split; ins; desf.
-  f_equal. now apply F_ID.
-Qed.
-
-Lemma partial_id_rel {A} (f : A -> option A) (r : relation A)
-    (F_ID : forall x y (SOME : f x = Some y), y = x) :
-  Some ↓ (f ↑ r) ≡ restr_rel (is_some ∘ f) r.
-Proof using.
-  symmetry.
-  unfolder. splits; ins; desf.
-  { do 2 eexists. rewrite <- !partial_id_iff; auto. }
-  rewrite (F_ID x' x), (F_ID y' y); splits; auto.
-  all: unfold is_some, compose; desf.
-Qed.
-
-Lemma partial_id_set {A} (f : A -> option A) (s : A -> Prop)
-    (F_ID : forall x y (SOME : f x = Some y), y = x) :
-  Some ↓₁ (f ↑₁ s) ≡₁ s ∩₁ (is_some ∘ f).
-Proof using.
-  symmetry.
-  unfolder. splits; ins; desf.
-  { eexists. rewrite <- !partial_id_iff; auto. }
-  rewrite (F_ID y x); auto.
-  all: unfold is_some, compose; desf.
-Qed.
-
-Lemma over_exec_wf f
-    (WF : Wf G')
-    (CTRL : ctrl' ≡ ∅₂)
-    (ADDR : addr' ≡ ∅₂)
-    (DATA : data' ≡ ∅₂)
-    (F_ID : forall x y (SOME : f x = Some y), y = x)
-    (A_CORRECT : is_some ∘ f ⊆₁ E)
-    (C_CORRECT : C ⊆₁ is_some ∘ f)
-    (SUB_INIT : E' ∩₁ is_init ⊆₁ E)
-    (G_RF_D : E ∩₁ R ⊆₁ codom_rel rf ∪₁ (Some ↓₁ (f ↑₁ C)))
-    (G_TIDS : ~(tid ↑₁ (E' ∩₁ set_compl is_init)) tid_init)
-    (G_ACTS : forall thr (NOT_INIT : thr <> tid_init),
-      exists N, E ∩₁ (fun x => thr = tid x) ≡₁ thread_seq_set thr N)
-    (SUB : sub_execution G' G ∅₂ ∅₂) :
-  WCore.wf (WCore.Build_t G G' C f).
-Proof using.
-  assert (ACT_SUB : E ∩₁ set_compl is_init ⊆₁ E' ∩₁ set_compl is_init).
-  { apply set_subset_inter; auto; apply SUB. }
-  constructor; ins.
-  { rewrite sub_ctrl, CTRL; eauto; basic_solver. }
-  { rewrite sub_addr, ADDR; eauto; basic_solver. }
-  { rewrite sub_data, DATA; eauto; basic_solver. }
-  { eapply sub_WF; eauto. now rewrite set_interC. }
-  { unfolder; intro INIT_IN; desf.
-    apply G_TIDS. eexists.
-    split; eauto; now apply ACT_SUB. }
-  { transitivity E; auto. apply SUB. }
-  { rewrite partial_id_set; eauto.
-    basic_solver. }
-  { unfolder; ins; desf.
-    apply F_ID. rewrite <- EQ.
-    now apply partial_id_iff. }
-  { rewrite sub_sb with (G' := G); eauto.
-    rewrite partial_id_rel, !restr_relE; auto.
-    basic_solver. }
-  { rewrite sub_rf with (G' := G); eauto.
-    rewrite partial_id_rel, !restr_relE; auto.
-    basic_solver. }
-  { unfolder. intros x y (HEQ & XIN & YIN).
-    apply F_ID in HEQ; now subst. }
-  { unfold WCore.unwrap_g2gc, same_lab_u2v_dom,
-          is_some, compose.
-    unfolder. ins. desf.
-    erewrite sub_lab, (F_ID e a); eauto.
-    red. desf. }
-  apply C_CORRECT, partial_id_iff in IN; auto.
-  unfold WCore.unwrap_g2gc, val.
-  erewrite sub_lab; eauto.
-  ins. now rewrite IN.
-Qed.
-
-End SubGraphLemma.
-
-Section ReorderingSubLemma.
-
-(* G ⊂ G' *)
-Definition delta_G G G' e :=
-  {| acts_set := acts_set G ∪₁ eq e;
-     threads_set := threads_set G;
-     lab := lab G;
-     rmw := rmw G ∪ (⦗acts_set G⦘ ⨾ (rmw G') ⨾ ⦗eq e⦘);
-     data := ∅₂;
-     addr := ∅₂;
-     ctrl := ∅₂;
-     rmw_dep := ⦗acts_set G ∪₁ eq e⦘ ⨾ rmw_dep G' ⨾ ⦗acts_set G ∪₁ eq e⦘;
-     rf := rf G ∪ (⦗acts_set G⦘ ⨾ (rf G') ⨾ ⦗eq e⦘) ∪
-                  (⦗eq e⦘ ⨾ (rf G') ⨾ ⦗acts_set G⦘);
-     co := co G ∪ (⦗acts_set G⦘ ⨾ (co G') ⨾ ⦗eq e⦘) ∪
-                  (⦗eq e⦘ ⨾ (co G') ⨾ ⦗acts_set G⦘);
-  |}.
-
-
-Variable G G' : execution.
-Variable C : actid -> Prop.
-Variable traces : thread_id -> trace label -> Prop.
-
-Notation "'lab''" := (lab G').
-Notation "'E''" := (acts_set G').
-Notation "'rmw''" := (rmw G').
-Notation "'data''" := (data G').
-Notation "'addr''" := (addr G').
-Notation "'ctrl''" := (ctrl G').
-Notation "'rmw_dep''" := (rmw_dep G').
-Notation "'rf''" := (rf G').
-Notation "'co''" := (co G').
-Notation "'W''" := (fun x => is_w lab' x).
-Notation "'R''" := (fun x => is_r lab' x).
-
-Notation "'lab'" := (lab G).
-Notation "'E'" := (acts_set G).
-Notation "'rmw'" := (rmw G).
-Notation "'data'" := (data G).
-Notation "'addr'" := (addr G).
-Notation "'ctrl'" := (ctrl G).
-Notation "'rmw_dep'" := (rmw_dep G).
-Notation "'rf'" := (rf G).
-Notation "'co'" := (co G).
-Notation "'W'" := (fun x => is_w lab x).
-Notation "'R'" := (fun x => is_r lab x).
-
-(* TODO: remove *)
-Notation "'U'" := (E' \₁ C).
-Notation "'D'" := (E' \₁ E).
-
-Lemma delta_G_sub e f
-    (NOT_INIT : tid e <> tid_init)
-    (WF : WCore.wf (WCore.Build_t G G' C f))
-    (IN : E' e)
-    (NEW : ~E e)
-    (SUB : sub_execution G' G ∅₂ ∅₂) :
-  sub_execution G' (delta_G G G' e) ∅₂ ∅₂.
-Proof using.
-  assert (WF' : Wf G').
-  { apply WF. }
-  assert (SUBE : E ⊆₁ E').
-  { apply SUB. }
-  constructor; ins.
-  all: try apply SUB.
-  { unfolder. ins. desf.
-    now apply SUB. }
-  { rewrite !id_union, seq_union_l,
-            !seq_union_r, <- (sub_rmw SUB).
-    rewrite one_dir_irrefl; eauto using rmw_one_dir.
-    destruct (classic (dom_rel (rmw' ⨾ ⦗E⦘) e)) as [HIN1|HIN1].
-    { rewrite one_dir_assym_1, !union_false_r;
-        eauto using rmw_one_dir, one_dir_dom.
-      unfolder in HIN1. desf.
-      enough (EINE : E e).
-      { arewrite (⦗eq e⦘ ≡ ⦗eq e⦘ ⨾ ⦗E⦘); try basic_solver. }
-      apply wf_rmwi, immediate_in in HIN1; eauto.
-      change E with (acts_set (WCore.G {|
-        WCore.G := G;
-        WCore.GC := G';
-        WCore.cmt := C;
-        WCore.g2gc := f
-      |})).
-      eapply WCore.ext_sb_dense; eauto.
-      unfold sb in HIN1. unfolder in HIN1.
-      desf. }
-    destruct (classic (codom_rel (⦗E⦘ ⨾ rmw') e)) as [HIN2|HIN2].
-    { rewrite one_dir_assym_2, !union_false_r;
-      eauto using rmw_one_dir, one_dir_dom. }
-    rewrite one_dir_assym_helper_1, one_dir_assym_helper_2,
-            !union_false_r; eauto. }
-  { rewrite (WCore.cc_data_empty WF); basic_solver. }
-  { rewrite (WCore.cc_addr_empty WF); basic_solver. }
-  { rewrite (WCore.cc_ctrl_empty WF); basic_solver. }
-  { rewrite !id_union, seq_union_l,
-            !seq_union_r, <- (sub_rf SUB).
-    rewrite one_dir_irrefl; eauto using rf_one_dir.
-    now rewrite union_false_r. }
-  { rewrite !id_union, seq_union_l,
-            !seq_union_r, <- (sub_co SUB).
-    arewrite (⦗eq e⦘ ⨾ co' ⨾ ⦗eq e⦘ ≡ ∅₂).
-    { set (IRR := co_irr WF').
-      unfold irreflexive in IRR.
-      split; [| basic_solver].
-      unfolder; ins; desf; eauto. }
-    now rewrite union_false_r. }
-  basic_solver.
-Qed.
-
-Hypothesis THREAD_EVENTS : forall t, exists N,
-  E' ∩₁ (fun e => t = tid e) ≡₁ thread_seq_set t N.
-
-Record reord_lemma_enum (E E' C : actid -> Prop) l : Prop :=
-{ relenum_nodup : NoDup l;
-  relenum_no_init : (fun x => In x l) ⊆₁ set_compl (fun a => is_init a);
-  relenum_d : (fun x => In x l) ≡₁ D;
-  relenum_sb : restr_rel (fun x => In x l) (sb G') ⊆ total_order_from_list l;
-  relenum_rf : restr_rel (fun x => In x l) rf' ⨾ ⦗E' \₁ C⦘ ⊆ total_order_from_list l;
-  relenum_rf_w : dom_rel (rf' ⨾ ⦗fun x => In x l⦘) ⊆₁ E ∪₁ fun x => In x l;
-}.
-
-(* TODO move to AuxDef.v *)
-Lemma equiv_seq_eq {A} (s : A -> Prop)
-  (r : relation A) :
-  ⦗s⦘ ⨾ (⦗s⦘ ⨾ r ⨾ ⦗s⦘) ⨾ ⦗s⦘ ≡ ⦗s⦘ ⨾ r ⨾ ⦗s⦘.
-Proof using.
-  basic_solver.
-Qed.
-
-Lemma sub_sym
-    (WF_G : Wf G')
-    (PREFIX : sub_execution G' G ∅₂ ∅₂)
-    (ENUM_D : D ≡₁ ∅)
-    : sub_execution G G' ∅₂ ∅₂.
-Proof using.
-    assert (E_EQ : E = E').
-    { apply set_extensionality.
-      split; eauto using sub_E.
-      now apply set_subsetE. }
-    constructor.
-    all: try now symmetry; apply PREFIX.
-    all: try now rewrite seq_false_l, seq_false_r.
-    { now rewrite E_EQ. }
-    all: rewrite 1?wf_rmwE,
-                 1?wf_dataE,
-                 1?wf_addrE,
-                 1?wf_ctrlE,
-                 1?wf_rmw_depE,
-                 1?wf_rfE,
-                 1?wf_coE; auto.
-    all: symmetry.
-    all: rewrite 1?sub_rmw,
-                 1?sub_data,
-                 1?sub_addr,
-                 1?sub_ctrl,
-                 1?sub_frmw,
-                 1?sub_rf,
-                 1?sub_co; eauto.
-    all: rewrite E_EQ.
-    all: apply equiv_seq_eq.
-Qed.
-
-Lemma sub_eq
-    (WF_G : Wf G')
-    (PREFIX : sub_execution G' G ∅₂ ∅₂)
-    (ENUM_D : D ≡₁ ∅)
-     : G = G'.
-Proof using.
-  eapply exec_equiv_eq, sub_sub_equiv; eauto.
-  now apply sub_sym.
-Qed.
-
-Lemma new_event_not_in_C e f
-    (WF : WCore.wf (WCore.Build_t G G' C f))
-    (NEW : D e) :
-  ~(Some ↓₁ (f ↑₁ C)) e.
-Proof using.
-  intro IN_C.
-  enough (E e) by now apply NEW.
-  apply (WCore.f_codom WF).
-  enough (Some ↓₁ (f ↑₁ C) ⊆₁ Some ↓₁ (f ↑₁ E')) by auto.
-  apply set_map_mori, set_subset_collect; eauto.
-  apply (WCore.C_sub_EC WF).
-Qed.
-
-(* NOTE: do not change threads_set! It must remain constant *)
-(* TODO: either rename or move into module *)
-Lemma step_once_read h t f
-    (F_ID : forall x y (SOME : f x = Some y), y = x)
-    (WF : WCore.wf (WCore.Build_t G G' C f))
-    (WF' : WCore.wf (WCore.Build_t G' G' C f))
-    (PREFIX : restr_exec E G' G)
-    (ENUM : reord_lemma_enum E E' C (h :: t))
-    (COH : trace_coherent traces G')
-    (IS_R : R' h) :
-  exists f' G'',
-    WCore.cfg_add_step_uninformative traces
-      (WCore.Build_t G   G' C f)
-      (WCore.Build_t G'' G' C f').
-Proof using THREAD_EVENTS.
-  assert (IN_D : D h).
-  { apply ENUM; now constructor. }
-  assert (NOT_W : ~ W' h).
-  { generalize IS_R. unfold is_w, is_r.
-    now destruct (lab' h). }
-  assert (R_IN_G' : (E' ∩₁ R') h).
-  { split; try apply IN_D; eauto. }
-  destruct (WCore.f_rfD WF' R_IN_G') as [RF | CMT]; ins.
-  all: try now (exfalso; eapply new_event_not_in_C with (f := f); eauto).
-  destruct RF as [w RF]; ins.
-  set (G'' := delta_G G G' h).
-  assert (G_SB_SUB : sb G ⊆ sb G'').
-  { unfold sb; subst G''; ins. basic_solver 2. }
-  assert (IS_W : W' w).
-  { eapply wf_rfD in RF; try now apply WF. unfolder in RF; desf. }
-  exists (upd f h (Some h)), G'',
-          h, (lab' h),
-          None, (Some w), ∅, ∅, (Some h).
-  constructor.
-  all: try easy.
-  all: ins; desf.
-  { apply IN_D. }
-  { apply ENUM; now constructor. }
-  { admit. }
-  { erewrite sub_lab with (G := G'); try apply PREFIX.
-    apply functional_extensionality; ins.
-    destruct (classic (x = h)) as [EQ|NEQ]; subst.
-    all: now rupd. }
-  { apply union_more; [apply union_more; auto |].
-    { admit. }
-    rewrite wf_rfD, seqA; try apply WF.
-    unfold WCore.rf_delta_W.
-    arewrite (⦗eq h⦘ ⨾ ⦗W'⦘ ≡ ∅₂); try basic_solver.
-    rewrite seq_false_l.
-    arewrite (upd f h (Some h) ↓₁ eq (Some h) ≡₁ eq h).
-    { unfolder; split; intros x HEQ; subst.
-      { destruct (classic (h = x)) as [EQ|NEQ]; auto.
-        rewrite updo in HEQ; auto. }
-      now rewrite upds. }
-    arewrite (⦗eq h⦘ ⨾ rf' ≡ ∅₂).
-    { rewrite wf_rfD; try apply WF'.
-      basic_solver. }
-    basic_solver. }
-  { admit. }
-  { admit. }
-  apply over_exec_wf.
-  all: try apply WF'.
-  { intros x y.
-    destruct (classic (x = h)) as [EQ|NEQ]; desf.
-    { rewrite upds; congruence. }
-    rewrite updo; auto. }
-  { unfolder. unfold is_some, compose. ins.
-    destruct (classic (x = h)) as [EQ|NEQ]; desf.
-    { now right. }
-    rewrite updo in Heq; auto.
-    left. apply (WCore.f_codom WF). ins.
-    assert (ID : f x = Some x) by now rewrite <- (F_ID x a) at 2.
-    exists x. split; [apply WF, partial_id_iff |]; auto. }
-  { transitivity (is_some ∘ f); try apply WF.
-    unfolder. unfold is_some, compose. ins.
-    destruct (classic (x = h)) as [EQ|NEQ]; desf.
-    { rewrite upds in Heq. congruence. }
-    rewrite updo in Heq; auto.
-    congruence. }
-  { subst G''. ins.
-    transitivity (E ∩₁ is_init); try apply PREFIX.
-    transitivity E; basic_solver. }
-  { subst G''. ins.
-    rewrite set_inter_union_l, codom_union.
-    admit.
-    (* split this into 2 refineable inclusions *) }
-  { subst G''. ins.
-    admit.
-    (* Infer it from trace coherency. *) }
-  subst G''. eapply delta_G_sub.
-  { admit. }
-  { apply WF. }
-  { apply IN_D. }
-  { apply IN_D. }
-  apply PREFIX.
-Admitted.
-
-Lemma step_once h t (f : actid -> option actid)
-  (WF : WCore.wf (WCore.Build_t G G' C f))
-  (PREFIX : restr_exec E G' G)
-  (C_SUB : C ⊆₁ E')
-  (VALID_ENUM : NoDup (h :: t))
-  (NOT_INIT : (fun x => In x (h :: t)) ⊆₁ set_compl is_init)
-  (ENUM_D : (fun x => In x (h :: t)) ≡₁ D)
-  (ORD_SB : restr_rel (fun x => In x (h :: t)) (sb G') ⊆ total_order_from_list (h :: t))
-  (ORD_RF : restr_rel (fun x => In x (h :: t)) rf' ⨾ ⦗U⦘ ⊆ total_order_from_list (h :: t)) :
-  exists f' G'',
-  (WCore.cfg_add_step_uninformative traces)
-  (WCore.Build_t G G' C f)
-  (WCore.Build_t G'' G' C f').
-Proof using.
-  eexists (upd f h (Some h)), _, h, (lab' h).
-  destruct (lab' h) eqn:HEQ_LAB.
-  all: admit.
-Admitted.
-
-(* Lemma steps l
-    (WF : Wf G)
-    (PREFIX : restr_exec E G' G)
-    (C_SUB : C ⊆₁ E')
-    (VALID_ENUM : NoDup l)
-    (ENUM_D : (fun x => In x l) ≡₁ D)
-    (ORD_SB : sb G' ⊆ enum_ord)
-    (ORD_RF : rf' ⨾ ⦗U⦘ ⊆ enum_ord) :
-    exists f',
-    (WCore.silent_cfg_add_step traces)＊
-    (WCore.Build_t G G' C f)
-    (WCore.Build_t G' G' C f').
-Proof using.
-  admit.
-Admitted. *)
-
-End ReorderingSubLemma.
 
 Section ReorderingLemmas.
 
